added subtyping

LeanCourse/Examples.lean
@@ -18,9 +18,10 @@ def StorageT  := Value Nat ValueSelector valSelector
 def StateType := State Nat ValueSelector valSelector IdTp
 def Selector  := FieldSelector ValueSelector valSelector
 def IdTyp     := IdT  ValueSelector valSelector IdTp
-def ValSTp  := ValT Nat ValueSelector valSelector IdTp
+def ValSTp    := ValT Nat ValueSelector valSelector IdTp
+def StructT   := Struct Nat ValueSelector valSelector
 
-variable (mem : MemT) (st : StorageT)
+variable (mem : MemT) (st : StructT)
 
 open Value
 open Memory
@@ -30,38 +31,40 @@ open Sum
 @[simp] def balance : Selector := .valS balanceS
 
 -- alice.account.balance = 10
-@[simp] def saveAlice : StorageT := save st [account, balance] $ var 10
+@[simp] def saveAlice : StorageT := save st.1 [account, balance] $ var 10
 
-theorem selectSaveAlice (isSt : isStruct st) : select (select (saveAlice st) account) balance = var 10 := by
+theorem selectSaveAlice : select (select (saveAlice st) account) balance = var 10 := by
   unfold saveAlice
-  have h := selectSave st account [balance] (var 10) account (by aesop)
+  have h := selectSave st.1 account [balance] (var 10) account st.2
   rewrite [h]
   simp
-  have h2 := selectSave (select st (FieldSelector.idS accountS))  balance [] (var 10) balance $ by aesop
+  have _ := st.2
+  have h2 := selectSave (select st.1 (FieldSelector.idS accountS))  balance [] (var 10) balance $ by aesop
   simp at h2
   rewrite [h2]
   simp
 
 -- alice.account.balance = 10
-@[simp] def stAlice : StorageT := store st account $ store mtst balance $ var 10
-@[simp] def stBob   : StorageT := store st account $ store mtst balance $ var 20
+@[simp] def stAlice : StorageT := store st.val account $ store mtst balance $ var 10
+@[simp] def stBob   : StorageT := store st.val account $ store mtst balance $ var 20
 -- idA = alice
-@[simp] def memAlice (_ : isStruct st := by aesop) := copySt mem idA (stAlice st) $ by aesop
+@[simp] def memAlice := copySt mem idA (stAlice st) $ by have _ := st.2; aesop
 
 
-theorem readCopy (_ : isStruct st := by aesop) : Memory.read (memAlice mem st) ⟨idA, [account]⟩ balance = .val 10
+theorem readCopy : Memory.read (memAlice mem st) ⟨idA, [account]⟩ balance = .val 10
  := by simp
 
-@[simp] def memBob (_ : isStruct st := by aesop) := copySt (memAlice mem st) idB (stBob st) $ by aesop
-@[simp] def idAA (_ : isStruct st := by aesop) := read (memBob mem st) ⟨idA, []⟩ account
-@[simp] def idBB (_ : isStruct st := by aesop) := read (memBob mem st) ⟨idB, []⟩ account
+@[simp] def memBob := copySt (memAlice mem st) idB (stBob st) $ by have _ := st.2; aesop
+@[simp] def idAA := read (memBob mem st) ⟨idA, []⟩ account
+@[simp] def idBB := read (memBob mem st) ⟨idB, []⟩ account
 
-theorem readIdAA (_ : isStruct st := by aesop) : idAA mem st = .id ⟨idA, [account]⟩ := by simp
-theorem readIdBB (_ : isStruct st := by aesop) : idBB mem st = .id ⟨idB, [account]⟩ := by simp
+theorem readIdAA : idAA mem st = .id ⟨idA, [account]⟩ := by simp
+theorem readIdBB : idBB mem st = .id ⟨idB, [account]⟩ := by simp
 
-theorem readIdABalance (_ : isStruct st := by aesop) : read (memBob mem st) ⟨idA, [account]⟩ balance
+theorem readIdABalance : read (memBob mem st) ⟨idA, [account]⟩ balance
   = .val 10  := by
   unfold memBob
+  have _ := st.2
   have h2 := readSkip (memAlice mem st) idB idA (stBob st)
   rewrite [h2]
   clear h2
@@ -71,7 +74,7 @@ theorem readIdABalance (_ : isStruct st := by aesop) : read (memBob mem st) ⟨i
   unfold copyStAux
   simp
 
-theorem readIdBBalance (_ : isStruct st := by aesop) : read (memBob mem st) ⟨idB, [account]⟩ balance = .val 20  := by simp
+theorem readIdBBalance : read (memBob mem st) ⟨idB, [account]⟩ balance = .val 20  := by simp
 
 -- -- acc.balance = n
 @[simp] def stAcc (n : Nat) : StorageT := store mtst balance $ var n
